Finish correctness proof for lifting.

theories/lang_oadt/lifting.v
@@ -146,6 +146,116 @@ Inductive lift_type_wf : list expr -> expr -> Prop :=
 
 Instance list_expr_stale : Stale (list expr) := foldr (fun e S => fv e ∪ S) ∅.
 
+(** ** Equivalence up to revelation *)
+
+(** [in_range τ τ' v] means value [v] of type [τ] is in the range of the
+oblivious type [τ']. In other words, it is constrained by the indices in τ'. *)
+Inductive in_range : expr -> expr -> expr -> Prop :=
+| IRSame τ v : in_range τ τ v
+| IRBool b : in_range <{ 𝔹 }> <{ ~𝔹 }> b
+| IRProd τ1 τ1' τ2 τ2' v1 v2 :
+    in_range τ1 τ1' v1 ->
+    in_range τ2 τ2' v2 ->
+    in_range <{ τ1 * τ2 }> <{ τ1' * τ2' }> <{ (v1, v2) }>
+| IRSum τ1 τ1' τ2 τ2' l b v :
+    in_range <{ ite b τ1 τ2 }> <{ ite b τ1' τ2' }> v ->
+    in_range <{ τ1 + τ2 }> <{ τ1' +{l} τ2' }> <{ inj@b<τ1 + τ2> v }>
+| IROADT X X' k v v' s r :
+    Δ !! (X, X') = Some (s, r) ->
+    (* We may want to use small-step semantics here instead, but it doesn't
+    matter: as reveal semantics is a weaker semantics and [in_range] is used in
+    assumptions, this formulation can only result in a stronger correctness
+    statement. *)
+    <{ (gvar s) k v }> ↓ v' ->
+    <{ (gvar r) k v' }> ↓ v ->
+    in_range <{ gvar X }> <{ X'@k }> v
+.
+
+
+(** We define the equivalence between a public expression and an oblivious
+expression up to revelation. The definition is essentially logical equivalence,
+but we do not treat higher-order arguments. The reason is rather subtle. *)
+
+(** [val_requiv τ τ' v v'] means value [v] of public type [τ] and [v'] of
+(possibly) oblivious type [τ'] are equivalent up to revelation. *)
+Inductive val_requiv : expr -> expr -> expr -> expr -> Prop :=
+| VQRefl τ v : val_requiv τ τ v v
+| VQBool b : val_requiv <{ 𝔹 }> <{ ~𝔹 }> <{ b }> <{ [b] }>
+| VQProd τ1 τ1' τ2 τ2' v1 v1' v2 v2' :
+    val_requiv τ1 τ1' v1 v1' ->
+    val_requiv τ2 τ2' v2 v2' ->
+    val_requiv <{ τ1 * τ2 }> <{ τ1' * τ2' }> <{ (v1, v2) }> <{ (v1', v2') }>
+| VQSum τ1 τ1' τ2 τ2' b v v' :
+    val_requiv <{ ite b τ1 τ2 }> <{ ite b τ1' τ2' }> v v' ->
+    val_requiv <{ τ1 + τ2 }> <{ τ1' + τ2' }>
+               <{ inj@b<τ1 + τ2> v }> <{ inj@b<τ1' + τ2'> v' }>
+| VQOSum τ1 τ1' τ2 τ2' ω1 ω2 b v v' :
+    val_requiv <{ ite b τ1 τ2 }> <{ ite b τ1' τ2' }> v v' ->
+    val_requiv <{ τ1 + τ2 }> <{ τ1' ~+ τ2' }>
+               <{ inj@b<τ1 + τ2> v }> <{ [inj@b<ω1 ~+ ω2> v'] }>
+| VQOADT X X' k v v' s r :
+    Δ !! (X, X') = Some (s, r) ->
+    <{ (gvar r) k v' }> ↓ v ->
+    val_requiv <{ gvar X }> <{ X'@k }> v v'
+.
+
+Section simple.
+
+(** This handles the case when at least one of the expressions has simple type,
+i.e. not function types. The top-level equivalence is defined parametric in this
+relation, so we can instantiate it with different semantics or equi-termination
+later. *)
+Variable expr_simple_requiv : expr -> expr -> expr -> expr -> Prop.
+
+(** Expression [e] of public type [τ] and [e'] of oblivious type [τ'] are
+equivalent up to revelation. *)
+Fixpoint expr_requiv_ (τ τ' : expr) (e e' : expr) : Prop :=
+  match τ, τ' with
+  | <{ Π:{_}τ1, τ2 }>, <{ Π:{_}τ1', τ2' }> =>
+    forall v v',
+      val v -> val v' ->
+      ∅ ⊢ v :{⊥} τ1 ->
+      ∅ ⊢ v' :{⊥} τ1' ->
+      val_requiv τ1 τ1' v v' ->
+      expr_requiv_ τ2 τ2' <{ e v }> <{ e' v' }>
+  | _, _ => expr_simple_requiv τ τ' e e'
+  end.
+
+(** [e] of public type [τ] and [e'] of oblivious type [τ'] with indices [τs] are
+equivalent up to revelation. Essentially this says [e] and [e'] are equivalent
+expressions, i.e. [expr_requiv], given any well-typed indices. *)
+Fixpoint lift_requiv_ (τs : list expr) (τ τ' : expr) (e e' : expr) : Prop :=
+  match τs with
+  | _::τs =>
+    match τ' with
+    | <{ Π:{_}τ1, τ2 }> =>
+      forall k : expr,
+        ∅ ⊢ k :{⊥} τ1 ->
+        val k ->
+        lift_requiv_ τs τ <{ τ2^k }> e <{ e' k }>
+    | _ => False
+    end
+  | [] => expr_requiv_ τ τ' e e'
+  end.
+
+End simple.
+
+(** This is the definitional equivalence, using the small-step semantics. Note
+that we only consider partial equivalence here, i.e. we assume they both
+terminate. Equi-termination can be handled separately. *)
+Definition expr_simple_requiv (τ τ' : expr) (e e' : expr) : Prop :=
+  forall w w',
+    e -->* w ->
+    wval w ->
+    in_range τ τ' (⟦w⟧) ->
+    e' -->* w' ->
+    wval w' ->
+    val_requiv τ τ' (⟦w⟧) (⟦w'⟧).
+
+Definition expr_requiv := expr_requiv_ expr_simple_requiv.
+Definition lift_requiv := lift_requiv_ expr_simple_requiv.
+
+
 (** * Theorems *)
 
 (** ** Well-typedness of section and retraction *)
@@ -293,6 +403,684 @@ Theorem lift_well_typed τs τ τ' e e' κ' :
   ∅ ⊢ e' :{⊥} τ'.
 Proof.
   eauto using lift_well_typed_.
+Qed.
+
+(** ** Stronger equivalence up to revelation *)
+
+(** This version of equivalence uses the reveal semantics [reval]. It is
+stronger than the definitional version, and much more convenient for proofs
+because we do not have to deal with weak values and the wacky semantics. *)
+Definition expr_simple_requiv_reval (τ τ' : expr) (e e' : expr) : Prop :=
+  forall v v',
+    e ↓ v ->
+    in_range τ τ' v ->
+    e' ↓ v' ->
+    val_requiv τ τ' v v'.
+
+Definition expr_requiv_reval := expr_requiv_ expr_simple_requiv_reval.
+Definition lift_requiv_reval := lift_requiv_ expr_simple_requiv_reval.
+
+Lemma expr_simple_requiv_reval_sound τ τ' e e' :
+  expr_simple_requiv_reval τ τ' e e' ->
+  expr_simple_requiv τ τ' e e'.
+Proof.
+  intros. hnf.
+  eauto using mstep_wval_reval.
+Qed.
+
+Lemma expr_requiv_reval_sound τ : forall τ' e e',
+  expr_requiv_reval τ τ' e e' ->
+  expr_requiv τ τ' e e'.
+Proof.
+  induction τ; cbn; intros;
+    try case_split; eauto using expr_simple_requiv_reval_sound.
+Qed.
+
+Lemma lift_requiv_reval_sound τs : forall τ τ' e e',
+    lift_requiv_reval τs τ τ' e e' ->
+    lift_requiv τs τ τ' e e'.
+Proof.
+  induction τs; cbn; intros;
+    try case_split; eauto; hauto use: expr_requiv_reval_sound.
+Qed.
+
+(** ** Substitution lemmas *)
+
+(** These lemmas are crucial to the proofs. They are used to keep terms closed
+throughout the proofs. Alternatively, we may use parallel substitution but it
+would need more work. *)
+
+Lemma gsec_subst_ τ τ' e e' x s :
+  lc s ->
+  gsec τ τ' e e' ->
+  gsec <{ {x↦s}τ }> <{ {x↦s}τ' }> <{ {x↦s}e }> <{ {x↦s}e' }>.
+Proof.
+  induction 2; simpl; econstructor; eauto;
+    (* GSCase *)
+    simpl_cofin;
+    match goal with
+    | H : ?R ?τ ?τ' _ _ |- ?R ?τ ?τ' _ _ =>
+      apply_eq H
+    end;
+    solve [ by rewrite subst_open_comm by (eauto; shelve)
+          | by rewrite subst_fresh by shelve ].
+
+  Unshelve.
+  all: fast_set_solver!!.
+Qed.
+
+Lemma gsec_subst τ τ' e e' x s :
+  gsec τ τ' e e' ->
+  lc s ->
+  x ∉ fv τ ∪ fv τ' ->
+  gsec τ τ' <{ {x↦s}e }> <{ {x↦s}e' }>.
+Proof.
+  intros.
+  apply_eq gsec_subst_; eauto;
+    by rewrite subst_fresh by fast_set_solver!!.
+Qed.
+
+Lemma gret_subst_type_neq τ τ' e' e x s :
+  gret τ τ' e' e ->
+  τ <> τ' ->
+  <{ {x↦s}τ }> <> <{ {x↦s}τ' }>.
+Proof.
+  induction 1; intros; try scongruence;
+    simpl_cofin?; hauto lq: on.
+Qed.
+
+Lemma gret_subst_ τ τ' e' e x s :
+  lc s ->
+  gret τ τ' e' e ->
+  gret <{ {x↦s}τ }> <{ {x↦s}τ' }> <{ {x↦s}e' }> <{ {x↦s}e }>.
+Proof.
+  induction 2; simpl; econstructor; eauto;
+    try match goal with
+        | H : _ <> _ |- _ <> _ =>
+            eapply gret_subst_type_neq in H; eauto using gret
+        end;
+    (* GRCase and GROCase *)
+    simpl_cofin;
+    match goal with
+    | H : ?R ?τ ?τ' _ _ |- ?R ?τ ?τ' _ _ =>
+      apply_eq H
+    end;
+    solve [ by rewrite subst_open_comm by (eauto; shelve)
+          | by rewrite subst_fresh by shelve ].
+
+  Unshelve.
+  all: fast_set_solver!!.
+Qed.
+
+Lemma gret_subst τ τ' e e' x s :
+  gret τ τ' e e' ->
+  lc s ->
+  x ∉ fv τ ∪ fv τ' ->
+  gret τ τ' <{ {x↦s}e }> <{ {x↦s}e' }>.
+Proof.
+  intros.
+  apply_eq gret_subst_; eauto;
+    by rewrite subst_fresh by fast_set_solver!!.
+Qed.
+
+Lemma lift_core_subst_ τ τ' e e' x s :
+  lc s ->
+  lift_core τ τ' e e' ->
+  lift_core <{ {x↦s}τ }> <{ {x↦s}τ' }> <{ {x↦s}e }> <{ {x↦s}e' }>.
+Proof.
+  induction 2; simpl in *; econstructor; eauto using gsec_subst_.
+  - simpl_cofin.
+    eapply_eq gret_subst_; eauto.
+    by rewrite subst_fresh by shelve.
+    by rewrite subst_open_comm by (eauto; shelve).
+  - simpl_cofin.
+    rewrite !subst_open_comm in * by (eauto; shelve).
+    eauto.
+
+  Unshelve.
+  all: fast_set_solver!!.
+Qed.
+
+Lemma lift_core_subst τ τ' e e' x s :
+  lift_core τ τ' e e' ->
+  lc s ->
+  x ∉ fv τ ∪ fv τ' ->
+  lift_core τ τ' <{ {x↦s}e }> <{ {x↦s}e' }>.
+Proof.
+  intros.
+  apply_eq lift_core_subst_; eauto;
+    by rewrite subst_fresh by fast_set_solver!!.
+Qed.
+
+Lemma lift_subst_ τs τ τ' e e' x s :
+  lc s ->
+  lift τs τ τ' e e' ->
+  x # τs ->
+  lift τs <{ {x↦s}τ }> <{ {x↦s}τ' }> <{ {x↦s}e }> <{ {x↦s}e' }>.
+Proof.
+  induction 2; intros; simpl in *.
+  - match goal with
+    | |- lift (?τ :: _) _ _ _ _ => rewrite (subst_fresh τ) by fast_set_solver!!
+    end.
+    econstructor. simpl_cofin.
+    rewrite <- !subst_open_comm by (auto; fast_set_solver!!).
+    auto_apply. fast_set_solver!!.
+  - econstructor.
+    eauto using lift_core_subst_.
+Qed.
+
+Lemma lift_subst τs τ τ' e e' x s :
+  lc s ->
+  lift τs τ τ' e e' ->
+  x ∉ stale τs ∪ fv τ ∪ fv e ->
+  lift τs τ <{ {x↦s}τ' }> e <{ {x↦s}e' }>.
+Proof.
+  intros.
+  apply_eq lift_subst_; eauto;
+    rewrite ?subst_fresh by fast_set_solver!!; eauto; fast_set_solver!!.
+Qed.
+
+(** ** Reveal semantics refinement *)
+
+Ltac apply_reval_deterministic :=
+  match goal with
+  | H : ?e ↓ ?v, H' : ?e ↓ ?v' |- _ =>
+      assert (v = v') by eauto using reval_deterministic;
+      simplify_eq; clear H
+  end.
+
+(** [e1] refines [e2]. *)
+Definition reval_refine (e1 e2 : expr) : Prop :=
+  forall v, e1 ↓ v -> e2 ↓ v.
+
+Instance reval_refine_preorder : PreOrder reval_refine.
+Proof.
+  split; hnf; unfold reval_refine.
+  - auto.
+  - auto.
+Qed.
+
+Lemma reval_refine_strengthen e e' :
+  (forall v, e ↓ v -> reval_refine e e') ->
+  reval_refine e e'.
+Proof.
+  unfold reval_refine.
+  eauto.
+Qed.
+
+Lemma reval_refine_reval1 e v :
+  e ↓ v ->
+  reval_refine e v.
+Proof.
+  intros. hnf. intros.
+  apply_reval_deterministic.
+  eauto using reval_idemp.
+Qed.
+
+Lemma reval_refine_reval2 e v :
+  e ↓ v ->
+  reval_refine v e.
+Proof.
+  intros. hnf. intros.
+  eapply reval_trans; eauto.
+Qed.
+
+Lemma reval_refine_erase1 e v :
+  reval_refine (⟦e⟧) v ->
+  reval_refine e v.
+Proof.
+  intros. hnf.
+  eauto using reval_erase, erase_idemp.
+Qed.
+
+Lemma reval_refine_erase2 e v :
+  reval_refine e (⟦v⟧) ->
+  reval_refine e v.
+Proof.
+  intros. hnf.
+  eauto using reval_erase, erase_idemp.
+Qed.
+
+Lemma reval_refine_congr_app e1 e2 s1 s2 :
+  reval_refine e1 e2 ->
+  reval_refine s1 s2 ->
+  reval_refine <{ e1 s1 }> <{ e2 s2 }>.
+Proof.
+  unfold reval_refine. intros.
+  reval_inv*. reval_intro; eauto.
+Qed.
+
+Lemma reval_refine_congr_app1 e1 e2 v :
+  reval_refine e1 e2 ->
+  reval_refine <{ e1 v }> <{ e2 v }>.
+Proof.
+  qauto use: reval_refine_congr_app solve: reflexivity.
+Qed.
+
+Lemma reval_refine_congr_app2 e1 e2 e :
+  reval_refine e1 e2 ->
+  reval_refine <{ e e1 }> <{ e e2 }>.
+Proof.
+  qauto use: reval_refine_congr_app solve: reflexivity.
+Qed.
+
+Lemma reval_refine_beta l τ e v :
+  val v ->
+  reval_refine <{ (\:{l}τ => e) v }> <{ e^v }>.
+Proof.
+  unfold reval_refine. intros.
+  reval_inv*.
+  select (val _) (fun H => eapply reval_val_inv in H); eauto; subst.
+  eauto using reval_erase, erase_open.
+Qed.
+
+Lemma reval_refine_beta_tape e :
+  reval_refine <{ tape e }> <{ e }>.
+Proof.
+  unfold reval_refine. intros.
+  reval_inv*. eauto.
+Qed.
+
+Lemma reval_refine_eta_prod e v1 v2 :
+  e ↓ <{ (v1, v2) }> ->
+  reval_refine e <{ (π1 e, π2 e) }>.
+Proof.
+  unfold reval_refine. intros.
+  apply_reval_deterministic.
+  econstructor; reval_intro; eauto.
+Qed.
+
+Lemma reval_refine_eta_prod_wt e l τ1 τ2 :
+  ∅ ⊢ e :{l} τ1 * τ2 ->
+  reval_refine e <{ (π1 e, π2 e) }>.
+Proof.
+  intros.
+  apply reval_refine_strengthen. intros.
+  select (_ ⊢ _ :{_} _ ) (fun H => eapply reval_soundness_strong in H);
+    eauto; simp_hyps.
+  select (val _) (fun H => eapply canonical_form_prod in H);
+    eauto; simp_hyps; subst.
+  eauto using reval_refine_eta_prod.
+Qed.
+
+Lemma reval_refine_eta_sum e b τ1 τ2 v :
+  e ↓ <{ inj@b<τ1 + τ2> v }> ->
+  lc τ1 -> lc τ2 ->
+  reval_refine e <{ case e of inl<τ1 + τ2> (bvar 0) | inr<τ1 + τ2> (bvar 0) }>.
+Proof.
+  unfold reval_refine. intros.
+  apply_reval_deterministic.
+  econstructor. eauto.
+  select (_ ↓ _) (fun H => apply reval_idemp in H).
+  reval_inv*. simpl.
+  rewrite !open_lc by eauto.
+  case_split; reval_intro; eauto; scongruence.
+Qed.
+
+(** ** Properties of equivalence-up-to-revelation *)
+
+Lemma expr_simple_requiv_reval_proper τ τ' e1 e2 e1' e2' :
+  expr_simple_requiv_reval τ τ' e1 e1' ->
+  reval_refine e2 e1 ->
+  reval_refine e2' e1' ->
+  expr_simple_requiv_reval τ τ' e2 e2'.
+Proof.
+  intros. hnf. eauto.
+Qed.
+
+Lemma expr_requiv_reval_proper τ : forall τ' e1 e2 e1' e2',
+  expr_requiv_reval τ τ' e1 e1' ->
+  reval_refine e2 e1 ->
+  reval_refine e2' e1' ->
+  expr_requiv_reval τ τ' e2 e2'.
+Proof.
+  induction τ; intros; simpl in *; eauto using expr_simple_requiv_reval_proper.
+  case_split; eauto using expr_simple_requiv_reval_proper.
+  intros. auto_eapply; eauto; eauto using reval_refine_congr_app1.
+Qed.
+
+Lemma lift_requiv_reval_proper τs : forall τ τ' e1 e2 e1' e2',
+  lift_requiv_reval τs τ τ' e1 e1' ->
+  reval_refine e2 e1 ->
+  reval_refine e2' e1' ->
+  lift_requiv_reval τs τ τ' e2 e2'.
+Proof.
+  induction τs; intros; simpl in *.
+  eapply expr_requiv_reval_proper; eauto.
+  case_split; eauto; intros.
+  auto_eapply; eauto; eauto using reval_refine_congr_app1.
+Qed.
+
+Instance expr_simple_requiv_reval_proper' τ τ' :
+  Proper (reval_refine ==> reval_refine ==> flip impl)
+         (expr_simple_requiv_reval τ τ').
+Proof.
+  repeat (intros; hnf).
+  eauto using expr_simple_requiv_reval_proper.
+Qed.
+
+Instance expr_requiv_reval_proper' τ τ' :
+  Proper (reval_refine ==> reval_refine ==> flip impl)
+         (expr_requiv_reval τ τ').
+Proof.
+  repeat (intros; hnf).
+  eapply expr_requiv_reval_proper; eauto.
+Qed.
+
+Instance lift_requiv_reval_proper' τs τ τ' :
+  Proper (reval_refine ==> reval_refine ==> flip impl)
+         (lift_requiv_reval τs τ τ').
+Proof.
+  repeat (intros; hnf).
+  eapply lift_requiv_reval_proper; eauto.
+Qed.
+
+Lemma val_requiv_same_type_ τ τ' e e' :
+  val_requiv τ τ' e e' ->
+  τ = τ' ->
+  e = e'.
+Proof.
+  induction 1; intros; simplify_eq; eauto;
+    try case_split; qauto.
+Qed.
+
+Lemma val_requiv_same_type τ e e' :
+  val_requiv τ τ e e' ->
+  e = e'.
+Proof.
+  eauto using val_requiv_same_type_.
+Qed.
+
+Lemma expr_simple_requiv_refl τ e :
+  expr_simple_requiv_reval τ τ e e.
+Proof.
+  hnf. intros.
+  apply_reval_deterministic.
+  econstructor.
+Qed.
+
+Lemma expr_requiv_refl τ : forall e,
+  expr_requiv_reval τ τ e e.
+Proof.
+  induction τ; simpl; intros; eauto using expr_simple_requiv_refl.
+  qauto use: val_requiv_same_type.
+Qed.
+
+Lemma expr_simple_requiv_strengthen τ τ' e e' :
+  (forall v v', e ↓ v ->
+           e' ↓ v' ->
+           in_range τ τ' v ->
+           expr_simple_requiv_reval τ τ' e e') ->
+  expr_simple_requiv_reval τ τ' e e'.
+Proof.
+  unfold expr_simple_requiv_reval.
+  eauto.
+Qed.
+
+Lemma expr_simple_requiv_congr_prod τ1 τ2 τ1' τ2' e1 e2 e1' e2' :
+  expr_simple_requiv_reval τ1 τ1' e1 e1' ->
+  expr_simple_requiv_reval τ2 τ2' e2 e2' ->
+  expr_simple_requiv_reval <{ τ1 * τ2 }> <{ τ1' * τ2' }>
+                           <{ (e1, e2) }> <{ (e1', e2') }>.
+Proof.
+  unfold expr_simple_requiv_reval.
+  intros. reval_inv*.
+  econstructor; eauto;
+    auto_apply; eauto;
+    qauto l: on inv: in_range ctrs: in_range.
+Qed.
+
+Lemma expr_simple_requiv_congr_osum τ1 τ2 τ1' τ2' b e e' τ τ3 τ4 :
+  expr_simple_requiv_reval <{ ite b τ1 τ2 }> <{ ite b τ1' τ2' }> e e' ->
+  expr_simple_requiv_reval <{ τ1 + τ2 }> <{ τ1' ~+ τ2' }>
+                           <{ inj@b<τ> e }> <{ ~inj@b<τ3 ~+ τ4> e' }>.
+Proof.
+  unfold expr_simple_requiv_reval.
+  intros. reval_inv*.
+  select (in_range _ _ _) (fun H => sinvert H).
+  econstructor; eauto.
+Qed.
+
+Lemma expr_simple_requiv_congr_case τ τ' e e1 e2 e1' e2' :
+  (forall v b τ0, e ↓ <{ inj@b<τ0> v }> ->
+             expr_simple_requiv_reval τ τ' <{ e1^v }> <{ e1'^v }>) ->
+  (forall v b τ0, e ↓ <{ inj@b<τ0> v }> ->
+             expr_simple_requiv_reval τ τ' <{ e2^v }> <{ e2'^v }>) ->
+  expr_simple_requiv_reval τ τ' <{ case e of e1 | e2 }> <{ case e of e1' | e2' }>.
+Proof.
+  unfold expr_simple_requiv_reval.
+  intros. reval_inv*.
+  apply_reval_deterministic.
+  case_split; eauto.
+Qed.
+
+(** ** Correctness of section and retraction *)
+
+Lemma gsec_reval_reflect τ τ' e e' v' :
+  gsec τ τ' e e' ->
+  e' ↓ v' ->
+  exists v, e ↓ v.
+Proof.
+  intros H. revert v'.
+  induction H; intros; reval_inv*; eauto.
+  select! (forall v, _ -> exists _, _) (fun H => edestruct H); eauto.
+  reval_inv*.
+  eauto.
+Qed.
+
+Lemma gsec_correct τ : forall τ' e e',
+  gsec τ τ' e e' ->
+  lc e ->
+  expr_simple_requiv_reval τ τ' e e'.
+Proof.
+  induction τ; intros ??? H; sinvert H; intros.
+  (* OADT *)
+  - hnf. intros. econstructor; eauto.
+    select (in_range _ _ _) (fun H => sinvert H).
+    simplify_map_eq.
+    match goal with
+    | H : ?e ↓ ?v, H' : <{ _ ?e }> ↓ _ |- _ =>
+        eapply reval_refine_congr_app2 in H';
+        eauto using reval_refine_reval1
+    end.
+    apply_reval_deterministic.
+    eauto.
+  (* Unit *)
+  - rewrite reval_refine_beta_tape.
+    apply expr_simple_requiv_refl.
+  (* Boolean *)
+  - rewrite reval_refine_beta_tape.
+    hnf. intros. reval_inv*.
+    apply_reval_deterministic.
+    econstructor.
+  (* Product *)
+  - apply expr_simple_requiv_strengthen; intros.
+    reval_inv*.
+    select! (gsec _ _ _ _)
+          (fun H => dup_hyp H (fun H => eapply gsec_reval_reflect in H)); eauto.
+    simp_hyps.
+    reval_inv*.
+    apply_reval_deterministic.
+    match goal with
+    | |- expr_simple_requiv_reval _ _ ?e _ =>
+        rewrite (reval_refine_eta_prod e) by eauto
+    end.
+    eapply expr_simple_requiv_congr_prod; auto_eapply; eauto using lc.
+  (* Oblivious Sum *)
+  - apply expr_simple_requiv_strengthen; intros.
+    reval_inv*.
+    select (in_range _ _ _) (fun H => sinvert H).
+    apply_reval_deterministic.
+    match goal with
+    | H : ?e ↓ _, H' : lc ?e |- _ =>
+        dup_hyp H (fun H => apply reval_lc in H); eauto
+    end.
+    repeat lc_inv.
+    rewrite reval_refine_beta_tape.
+    match goal with
+    | |- expr_simple_requiv_reval _ _ ?e _ =>
+        rewrite (reval_refine_eta_sum e) at 1 by eauto
+    end.
+    simpl_cofin.
+    repeat
+      match goal with
+      | H : gsec _ _ <{ fvar ?x }> _, H' : _ ↓ <{ inj@_<_> ?v }> |- _ =>
+          eapply gsec_subst with (x:=x) (s:=v) in H;
+          [ simpl in H;
+            rewrite decide_True in H by auto;
+            rewrite <- subst_intro in H by fast_set_solver!!
+          | eauto | fast_set_solver!! ]
+      end.
+    eapply expr_simple_requiv_congr_case; intros;
+      apply_reval_deterministic; simpl;
+      eauto using expr_simple_requiv_congr_osum.
+Qed.
+
+Lemma gret_correct_ τ τ' v v' :
+  val_requiv τ τ' v v' ->
+  forall e e',
+    gret τ τ' e' e ->
+    lc τ -> lc e' ->
+    e' ↓ ⟦v'⟧ ->
+    e ↓ ⟦v⟧.
+Proof.
+  induction 1; intros;
+    select (gret _ _ _ _) (fun H => sinvert H);
+    eauto; try solve [ exfalso; eauto ];
+    repeat
+      match goal with
+      | H : val_requiv ?τ ?τ _ _ |- _ =>
+          eapply val_requiv_same_type in H; subst
+      end; eauto;
+    match goal with
+    | H : ?e ↓ _, H' : lc ?e |- _ =>
+        dup_hyp H (fun H => apply reval_lc in H); eauto
+    end;
+    simpl in *; repeat lc_inv.
+  (* [VQBool] *)
+  - econstructor.
+    hauto ctrs: reval, oval.
+    hauto ctrs: reval, val.
+  (* [VQProd] *)
+  - econstructor; auto_eapply; eauto using lc;
+      reval_intro; eauto.
+  (* [VQSum] *)
+  - econstructor; eauto.
+    simpl. rewrite !open_lc by eauto.
+    simpl_cofin.
+    repeat
+      match goal with
+      | H : gret _ _ <{ fvar ?x }> _, H' : _ ↓ <{ inj@_<_> ?v }> |- _ =>
+          eapply gret_subst with (x:=x) (s:=v) in H;
+          [ simpl in H;
+            rewrite decide_True in H by auto;
+            rewrite <- subst_intro in H by fast_set_solver!!
+          | eauto | fast_set_solver!! ]
+      end.
+    select (_ ↓ <{ inj@_<_> _ }>) (fun H => apply reval_idemp in H).
+    reval_inv*.
+    case_split; econstructor; auto_eapply; eauto.
+  (* [VQOSum] *)
+  - econstructor; eauto using reval, oval.
+    simpl. rewrite !open_lc by eauto.
+    simpl_cofin.
+    repeat
+      match goal with
+      | H : gret _ _ <{ fvar ?x }> _, H' : _ ↓ <{ [inj@_<_> ?v] }> |- _ =>
+          eapply gret_subst with (x:=x) (s:=v) in H;
+          [ simpl in H;
+            rewrite decide_True in H by auto;
+            rewrite <- subst_intro in H by fast_set_solver!!
+          | eauto with lc | fast_set_solver!! ]
+      end.
+    case_split; econstructor; auto_eapply; eauto using reval, oval_val with lc.
+  (* VQOADT *)
+  - erewrite <- reval_fix_erase by eauto.
+    eapply reval_refine_congr_app2; eauto.
+    eauto using reval_refine_erase1, reval_refine_reval2.
+Qed.
+
+Lemma gret_correct τ τ' v v' e :
+  val_requiv τ τ' v v' ->
+  gret τ τ' v' e ->
+  lc τ -> lc v' ->
+  val v' ->
+  e ↓ ⟦v⟧.
+Proof.
+  intros.
+  eapply gret_correct_; eauto using reval.
+Qed.
+
+(** ** Correctness of lifting *)
+
+Lemma gret_lc τ τ' e e' :
+  gret τ τ' e e' ->
+  lc τ ->
+  lc τ' ->
+  lc e ->
+  lc e'.
+Proof.
+  induction 1; intros; repeat lc_inv; eauto 10 using lc;
+    (* Sum and Oblivious sum *)
+    econstructor; eauto using lc;
+    simpl_cofin; simpl;
+    rewrite !open_lc by eauto;
+    eauto 10 using lc.
+Qed.
+
+Lemma lift_core_correct τ : forall τ' e e',
+  lift_core τ τ' e e' ->
+  lc e ->
+  expr_requiv_reval τ τ' e e'.
+Proof.
+  induction τ; intros ??? H; sinvert H; simpl; intros;
+    eauto using gsec_correct;
+    try qauto l: on inv: gsec.
+
+  simpl_cofin.
+  let go H lem x v :=
+    eapply lem with (x:=x) (s:=v) in H;
+    [ | eauto with lc | fast_set_solver!! ];
+    simpl in H;
+    rewrite ?decide_True in H by eauto;
+    rewrite <- ?subst_intro in H by eauto;
+    rewrite ?subst_fresh in H by eauto
+        in match goal with
+     | H : gret _ _ <{ fvar ?x }> _, H' : lift_core _ _ _ _ |-
+         expr_requiv_reval _ _ _ <{ _ ?v }> =>
+         go H gret_subst x v;
+         go H' lift_core_subst x v
+     end.
+  rewrite reval_refine_beta by eauto.
+  rewrite reval_refine_congr_app2.
+  - eauto 10 using gret_lc with lc.
+  - eauto 10 using gret_correct, reval_refine_erase1, reval_refine_reval2 with lc.
+Qed.
+
+Lemma lift_correct_ τs : forall τ τ' e e',
+  lift τs τ τ' e e' ->
+  lc e ->
+  lift_requiv_reval τs τ τ' e e'.
+Proof.
+  induction τs; intros ???? H; sinvert H; simpl; intros.
+  - eapply lift_core_correct; eauto.
+  - simpl_cofin.
+    match goal with
+    | H : lift _ _ _ _ <{ _^(fvar ?x) }> |- lift_requiv_reval _ _ _ _ <{ _ ?v }> =>
+        eapply lift_subst with (x:=x) (s:=v) in H;
+        [ | eauto with lc | fast_set_solver!! ];
+        rewrite <- ?subst_intro in H by eauto
+    end.
+    rewrite reval_refine_beta by eauto.
+    eauto.
+Qed.
+
+Theorem lift_correct τs τ τ' e e' :
+  lift τs τ τ' e e' ->
+  lc e ->
+  lift_requiv τs τ τ' e e'.
+Proof.
+  eauto using lift_correct_, lift_requiv_reval_sound.
 Qed.
 
 End lifting.
